src/lib/communication/DY.Lib.Communication.RequestResponse.Lemmas.fst
@@ -19,43 +19,28 @@ open DY.Lib.Communication.RequestResponse.Invariants
 
 (*** Lemmas ***)
 
-val is_comm_response_payload: {|crypto_invariants|} -> trace -> principal -> comm_meta_data -> bytes -> prop
-let is_comm_response_payload #cusg tr server req_meta_data payload =
-  bytes_invariant tr payload /\
-  get_label tr payload `can_flow tr` get_label #default_crypto_usages tr req_meta_data.key /\
-  bytes_well_formed tr payload
-
 val get_response_label: tr:trace -> comm_meta_data -> label
 let get_response_label tr req_meta_data = get_label #default_crypto_usages tr req_meta_data.key
+
+val is_comm_response_payload:
+  {|crypto_invariants|} ->
+  #a:Type -> {| parseable_serializeable bytes a |} ->
+  trace -> principal -> comm_meta_data -> a -> prop
+let is_comm_response_payload #cusg #a tr server req_meta_data payload =
+  is_well_formed a (is_knowable_by (get_response_label tr req_meta_data) tr) payload
 
 val comm_meta_data_knowable: {|crypto_invariants|} -> trace -> principal -> comm_meta_data -> prop
 let comm_meta_data_knowable #cinvs tr prin req_meta_data =
   is_knowable_by (principal_label prin) tr req_meta_data.key
 
 
-val compute_request_message_proof:
-  {|crypto_invariants|} ->
-  tr:trace ->
-  client:principal -> server:principal ->
-  payload:bytes -> key:bytes ->
-  Lemma
-  (requires
-    is_secret (comm_label client server) tr key /\
-    is_knowable_by (comm_label client server) tr payload
-  )
-  (ensures
-    is_knowable_by (comm_label client server) tr (compute_request_message payload key)
-  )
-let compute_request_message_proof #invs tr client server payload key =
-  serialize_wf_lemma request_message (is_knowable_by (comm_label client server) tr) {payload; key};
-  ()
-
 val send_request_proof:
   {|protocol_invariants|} ->
+  #a:Type -> {| parseable_serializeable bytes a |} ->
   tr:trace ->
   comm_keys_ids:communication_keys_sess_ids ->
-  higher_layer_preds:comm_reqres_higher_layer_event_preds ->
-  client:principal -> server:principal -> payload:bytes ->
+  higher_layer_preds:comm_reqres_higher_layer_event_preds a ->
+  client:principal -> server:principal -> payload:a ->
   Lemma
   (requires
     trace_invariant tr /\
@@ -64,34 +49,36 @@ val send_request_proof:
     has_communication_layer_reqres_event_predicates request_response_event_preconditions higher_layer_preds /\
     has_communication_layer_state_predicates /\
     higher_layer_preds.send_request tr client server payload (comm_label client server) /\
-    is_knowable_by (comm_label client server) tr payload
+    is_well_formed a (is_knowable_by (comm_label client server) tr) payload
   )
   (ensures (
     let (_, tr_out) = send_request comm_keys_ids client server payload tr in
     trace_invariant tr_out
   ))
-let send_request_proof #invs tr comm_keys_ids higher_layer_preds client server payload =
+let send_request_proof #invs #a tr comm_keys_ids higher_layer_preds client server payload =
+  let payload_bytes = serialize #bytes a payload in
   match send_request comm_keys_ids client server payload tr with
   | (None, tr_out) -> (
     let (key, tr') = mk_rand (AeadKey comm_layer_aead_tag empty) (comm_label client server) 32 tr in
     let (id, tr') = mk_rand NoUsage (comm_label client server) 32 tr' in
     let (sid, tr') = new_session_id client tr' in
-    let ((), tr') = set_state client sid (ClientSendRequest {server; payload; key} <: communication_states) tr' in
+    let ((), tr') = set_state client sid (ClientSendRequest {server; payload=payload_bytes; key} <: communication_states) tr' in
     higher_layer_preds.send_request_later tr tr' client server payload (get_label tr' key);
-    let ((), tr') = trigger_event client (CommClientSendRequest client server payload key) tr' in
+    let ((), tr') = trigger_event client (CommClientSendRequest client server payload_bytes key) tr' in
     ()
   )
   | (Some _, tr_out) -> (
     let (key, tr') = mk_rand (AeadKey comm_layer_aead_tag empty) (comm_label client server) 32 tr in
-    let (id, tr') = mk_rand NoUsage (comm_label client server) 32 tr' in
+    let (id, tr') = mk_rand NoUsage (comm_label client server) 32 tr' in    
     let (sid, tr') = new_session_id client tr' in
-    let ((), tr') = set_state client sid (ClientSendRequest {server; payload; key} <: communication_states) tr' in
+    let ((), tr') = set_state client sid (ClientSendRequest {server; payload=payload_bytes; key} <: communication_states) tr' in
     higher_layer_preds.send_request_later tr tr' client server payload (get_label tr' key);
-    let ((), tr') = trigger_event client (CommClientSendRequest client server payload key) tr' in
-    compute_request_message_proof tr' client server payload key;
-    let req_payload = compute_request_message payload key in
-    send_confidential_proof #invs tr' request_response_event_preconditions comm_keys_ids client server req_payload;   
-    let (Some msg_id, tr') = send_confidential comm_keys_ids client server req_payload tr' in
+    let ((), tr') = trigger_event client (CommClientSendRequest client server payload_bytes key) tr' in
+    assert(trace_invariant tr');
+    let req_payload:request_message = {payload=(serialize a payload); key} in
+    let req_payload_bytes = serialize #bytes request_message req_payload in
+    send_confidential_proof #invs #request_message tr' request_response_event_preconditions comm_keys_ids client server req_payload;   
+    let (Some msg_id, tr') = send_confidential #request_message comm_keys_ids client server req_payload tr' in
 
     assert(tr_out == tr');
     assert(trace_invariant tr_out);
@@ -99,43 +86,13 @@ let send_request_proof #invs tr comm_keys_ids higher_layer_preds client server p
   )
 
 
-val decode_request_message_proof:
-  {|crypto_invariants|} ->
-  tr:trace ->
-  server:principal -> msg_bytes:bytes ->
-  Lemma
-  (requires
-    exists client. is_knowable_by (comm_label client server) tr msg_bytes
-  )
-  (ensures (
-    match decode_request_message msg_bytes with
-    | None -> True
-    | Some {payload; key} -> (
-      exists client.
-        is_knowable_by (comm_label client server) tr payload /\
-        is_knowable_by (comm_label client server) tr key
-    )
-  ))
-let decode_request_message_proof #cinvs tr server msg_bytes =
-  match decode_request_message msg_bytes with
-  | None -> ()
-  | Some {payload; key} -> (
-    eliminate exists client. is_knowable_by (comm_label client server) tr msg_bytes
-    returns (exists client.
-        is_knowable_by (comm_label client server) tr payload /\
-        is_knowable_by (comm_label client server) tr key)
-    with _. (
-      parse_wf_lemma request_message (is_knowable_by (comm_label client server) tr) msg_bytes;
-     ()
-    )
-  )
-
-#push-options "--z3rlimit 20"
+#push-options "--z3rlimit 50"
 val receive_request_proof:
   {|protocol_invariants|} ->
+  #a:Type -> {| parseable_serializeable bytes a |} ->
   tr:trace ->
   comm_keys_ids:communication_keys_sess_ids ->
-  higher_layer_preds:comm_reqres_higher_layer_event_preds ->
+  higher_layer_preds:comm_reqres_higher_layer_event_preds a ->
   server:principal -> msg_id:timestamp ->
   Lemma
   (requires
@@ -147,29 +104,34 @@ val receive_request_proof:
     has_communication_layer_state_predicates
   )
   (ensures (
-    match receive_request comm_keys_ids server msg_id tr with
+    match receive_request #a comm_keys_ids server msg_id tr with
     | (None, tr_out) -> trace_invariant tr_out
     | (Some (payload, req_meta_data), tr_out) -> (
+      let payload_bytes = serialize a payload in
       trace_invariant tr_out /\
-      event_triggered tr_out server (CommServerReceiveRequest server payload req_meta_data.key) /\    
+      // See comment on `receive_confidential_proof` for the reason of this form
+      // of the post-condition.
+      (exists client. event_triggered tr_out client (CommClientSendRequest client server payload_bytes req_meta_data.key) \/
+        is_well_formed a (is_publishable tr_out) payload) /\
+      is_well_formed a (is_knowable_by (principal_label server) tr_out) payload /\
       is_comm_response_payload tr_out server req_meta_data payload
     )
   ))
-let receive_request_proof #invs tr comm_keys_ids higher_layer_preds server msg_id =
-  match receive_request comm_keys_ids server msg_id tr with
+let receive_request_proof #invs #a tr comm_keys_ids higher_layer_preds server msg_id =
+  receive_confidential_proof #invs tr request_response_event_preconditions comm_keys_ids server msg_id;
+  match receive_request #a comm_keys_ids server msg_id tr with
   | (None, tr_out) -> ()
   | (Some (payload, req_meta_data), tr_out) -> (
-    receive_confidential_proof #invs tr request_response_event_preconditions comm_keys_ids server msg_id;
-    let (Some req_msg_bytes, tr') = receive_confidential comm_keys_ids server msg_id tr in
-    decode_request_message_proof tr' server req_msg_bytes;
-    let Some req_msg = decode_request_message req_msg_bytes in    
-    FStar.Classical.move_requires (parse_wf_lemma request_message (is_publishable tr')) req_msg_bytes;
+    let (Some req_msg, tr') = receive_confidential #request_message comm_keys_ids server msg_id tr in
+
+    serialize_parse_inv_lemma #bytes a req_msg.payload;
+    assert(is_comm_response_payload tr_out server req_meta_data payload);
+
     let ((), tr') = trigger_event server (CommServerReceiveRequest server req_msg.payload req_msg.key) tr' in
     let (sid', tr') = new_session_id server tr' in
     let ((), tr') = set_state server sid' (ServerReceiveRequest {payload=req_msg.payload; key=req_msg.key} <: communication_states) tr' in
-    
-    assert(tr' == tr_out);
-    assert(trace_invariant tr_out);   
+    assert(tr' == tr_out);    
+    assert(trace_invariant tr_out);
     ()
   )
 #pop-options
@@ -190,7 +152,7 @@ val mk_comm_layer_response_nonce_proof:
     match mk_comm_layer_response_nonce server req_meta_data usg tr with
     | (None, tr_out) -> trace_invariant tr_out
     | (Some nonce, tr_out) -> (
-      is_comm_response_payload tr_out server req_meta_data nonce
+      is_knowable_by (get_response_label tr_out req_meta_data) tr_out nonce
     )
   ))
 let mk_comm_layer_response_nonce_proof #invs tr server req_meta_data usg = ()
@@ -198,27 +160,27 @@ let mk_comm_layer_response_nonce_proof #invs tr server req_meta_data usg = ()
 
 val compute_response_message_proof:
   {|crypto_invariants|} ->
+  #a:Type -> {| parseable_serializeable bytes a |} ->
   tr:trace ->
   server:principal ->
-  key:bytes -> nonce:bytes -> payload:bytes ->
+  key:bytes -> nonce:bytes -> payload:a ->
   Lemma
   (requires
     has_communication_layer_reqres_crypto_predicates /\
     is_knowable_by (principal_label server) tr key /\
-    is_knowable_by (get_label tr key) tr payload /\    
+    is_well_formed a (is_knowable_by (get_label tr key) tr) payload /\    
     is_publishable tr nonce /\
     (key `has_usage tr` (AeadKey comm_layer_aead_tag empty) \/
       is_publishable tr key    
     ) /\
-    event_triggered tr server (CommServerSendResponse server payload)
+    event_triggered tr server (CommServerSendResponse server (serialize a payload))
   )
   (ensures
-    is_publishable tr (compute_response_message server key nonce payload)
+    is_publishable tr (compute_response_message #a server key nonce payload)
   )
-let compute_response_message_proof #cinvs tr server key nonce payload =
-  let res:response_message = {payload} in
-  let res_bytes = serialize response_message res in
-  serialize_wf_lemma response_message (is_knowable_by (get_label tr key) tr) res;
+let compute_response_message_proof #cinvs #a tr server key nonce payload =
+  let res_bytes = serialize a payload in
+  serialize_wf_lemma a (is_knowable_by (get_label tr key) tr) payload;
   let ad:authenticated_data = {server} in
   let ad_bytes = serialize authenticated_data ad in
   serialize_wf_lemma authenticated_data (is_publishable tr) ad;
@@ -230,10 +192,11 @@ let compute_response_message_proof #cinvs tr server key nonce payload =
 
 val send_response_proof:
   {|protocol_invariants|} ->
+  #a:Type -> {| parseable_serializeable bytes a |} ->
   tr:trace ->
   comm_keys_ids:communication_keys_sess_ids ->
-  higher_layer_preds:comm_reqres_higher_layer_event_preds ->
-  server:principal -> req_meta_data:comm_meta_data -> payload:bytes ->
+  higher_layer_preds:comm_reqres_higher_layer_event_preds a ->
+  server:principal -> req_meta_data:comm_meta_data -> payload:a ->
   Lemma
   (requires
     trace_invariant tr /\
@@ -244,16 +207,16 @@ val send_response_proof:
     is_comm_response_payload tr server req_meta_data payload
   )
   (ensures (
-    let (_, tr_out) = send_response comm_keys_ids server req_meta_data payload tr in
+    let (_, tr_out) = send_response #a comm_keys_ids server req_meta_data payload tr in
     trace_invariant tr_out
   ))
-let send_response_proof #invs tr comm_keys_ids higher_layer_preds server req_meta_data payload =
+let send_response_proof #invs #a tr comm_keys_ids higher_layer_preds server req_meta_data payload =
   match send_response comm_keys_ids server req_meta_data payload tr with
   | (None, tr_out) -> ()
   | (Some msg_id, tr_out) -> (
     let (Some state, tr') = get_state server req_meta_data.sid tr in
     let ServerReceiveRequest srr = state in    
-    let ((), tr') = trigger_event server (CommServerSendResponse server payload) tr' in    
+    let ((), tr') = trigger_event server (CommServerSendResponse server (serialize a payload)) tr' in    
     let (nonce, tr') = mk_rand NoUsage public 32 tr' in
     compute_response_message_proof tr' server req_meta_data.key nonce payload;
     let resp_msg_bytes = compute_response_message server req_meta_data.key nonce payload in
@@ -267,6 +230,7 @@ let send_response_proof #invs tr comm_keys_ids higher_layer_preds server req_met
 #push-options "--fuel 0 --ifuel 1 --z3rlimit 10"
 val decode_response_proof:
   {|crypto_invariants|} ->
+  #a:Type -> {| parseable_serializeable bytes a |} ->
   tr:trace ->
   client:principal -> server:principal ->
   key:bytes -> msg_bytes:bytes ->
@@ -278,16 +242,17 @@ val decode_response_proof:
     key `has_usage tr` (AeadKey comm_layer_aead_tag empty)
   )
   (ensures (
-    match decode_response_message server key msg_bytes with
+    match decode_response_message #a server key msg_bytes with
     | None -> True
     | Some payload -> (
-      is_knowable_by (get_label tr key) tr payload /\
-      (event_triggered tr server (CommServerSendResponse server payload)
+      is_well_formed a (is_knowable_by (get_label tr key) tr) payload /\
+      is_knowable_by (get_label tr key) tr (serialize a payload) /\
+      (event_triggered tr server (CommServerSendResponse server (serialize a payload))
         \/ is_corrupt tr (principal_label client) \/ is_corrupt tr (principal_label server))
     )
   ))
-let decode_response_proof #cinvs tr client server key msg_bytes =
-  match decode_response_message server key msg_bytes with
+let decode_response_proof #cinvs #a #ps tr client server key msg_bytes =
+  match decode_response_message #a server key msg_bytes with
   | None -> ()
   | Some payload -> (
     parse_wf_lemma response_envelope (is_publishable tr) msg_bytes;
@@ -295,16 +260,17 @@ let decode_response_proof #cinvs tr client server key msg_bytes =
     serialize_wf_lemma authenticated_data (is_publishable tr) {server};
     let ad_bytes = serialize authenticated_data {server} in
     let Some res_bytes = aead_dec key nonce ciphertext ad_bytes in
-    parse_wf_lemma response_message (is_knowable_by (comm_label client server) tr) res_bytes;
+    serialize_parse_inv_lemma #bytes a #ps res_bytes;
     ()
   )
 #pop-options
 
 val receive_response_proof:
   {|protocol_invariants|} ->
+  #a:Type -> {| parseable_serializeable bytes a |} ->
   tr:trace ->
   comm_keys_ids:communication_keys_sess_ids ->
-  higher_layer_preds:comm_reqres_higher_layer_event_preds ->
+  higher_layer_preds:comm_reqres_higher_layer_event_preds a ->
   client:principal -> req_meta_data:comm_meta_data -> msg_id:timestamp ->
   Lemma
   (requires
@@ -316,15 +282,16 @@ val receive_response_proof:
     has_communication_layer_state_predicates
   )
   (ensures (
-    match receive_response comm_keys_ids client req_meta_data msg_id tr with
+    match receive_response #a comm_keys_ids client req_meta_data msg_id tr with
     | (None, tr_out) -> trace_invariant tr_out
     | (Some (payload, _), tr_out) -> (
       trace_invariant tr_out /\
-      event_triggered tr_out client (CommClientReceiveResponse client req_meta_data.server payload req_meta_data.key)
+      event_triggered tr_out client (CommClientReceiveResponse client req_meta_data.server (serialize a payload) req_meta_data.key) /\
+      is_well_formed a (is_knowable_by (get_label tr req_meta_data.key) tr) payload
     )
   ))
-let receive_response_proof #invs tr comm_keys_ids higher_layer_preds client req_meta_data msg_id =
-  match receive_response comm_keys_ids client req_meta_data msg_id tr with
+let receive_response_proof #invs #a tr comm_keys_ids higher_layer_preds client req_meta_data msg_id =
+  match receive_response #a comm_keys_ids client req_meta_data msg_id tr with
   | (None, tr_out) -> ()
   | (Some (payload, _), tr_out) -> (
     let server = req_meta_data.server in
@@ -332,11 +299,11 @@ let receive_response_proof #invs tr comm_keys_ids higher_layer_preds client req_
     let (Some state, tr') = get_state client req_meta_data.sid tr in
     let ClientSendRequest csr = state in
     let (Some resp_msg_bytes, tr') = recv_msg msg_id tr' in
-    decode_response_proof tr' client csr.server csr.key resp_msg_bytes;
-    let Some payload = decode_response_message csr.server csr.key resp_msg_bytes in
-    let ((), tr') = set_state client req_meta_data.sid (ClientReceiveResponse {server=csr.server; payload; key=csr.key} <: communication_states) tr' in
-    let ((), tr') = trigger_event client (CommClientReceiveResponse client csr.server payload csr.key) tr' in
-
+    decode_response_proof #invs.crypto_invs #a tr' client csr.server csr.key resp_msg_bytes;
+    let Some payload = decode_response_message #a csr.server csr.key resp_msg_bytes in
+    let ((), tr') = set_state client req_meta_data.sid (ClientReceiveResponse {server=csr.server; payload=(serialize a payload); key=csr.key} <: communication_states) tr' in
+    let ((), tr') = trigger_event client (CommClientReceiveResponse client csr.server (serialize a payload) csr.key) tr' in
+    assert(event_triggered tr' client (CommClientReceiveResponse client csr.server (serialize a payload) csr.key));
     assert(tr_out == tr');
     assert(trace_invariant tr_out);
     ()
